unity/predicate.lean
@@ -1,0 +1,30 @@
+
+
+namespace predicate
+
+def pred' α := α → Prop
+
+def False {α} : pred' α := λ_, false
+def True {α} : pred' α := λ_, true
+
+@[reducible]
+def p_or {α} (p₀ p₁ : pred' α) : pred' α
+:= λx, p₀ x ∨ p₁ x
+
+@[reducible]
+def p_and {α} (p₀ p₁ : pred' α) : pred' α
+:= λx, p₀ x ∧ p₁ x
+
+def p_impl {α} (p₀ p₁ : pred' α) : pred' α
+:= λx, p₀ x → p₁ x
+
+def p_not {α} (p : pred' α) : pred' α
+:= λx, ¬ p x
+
+infixl ` || ` := p_or
+infixl ` && ` := p_and
+infixl ` ⟶ `:60 := p_impl
+
+notation `~`:1 x := p_not x
+
+end predicate
