unity/safety.lean
@@ -1,0 +1,90 @@
+
+import unity.predicate
+
+import util.logic
+
+namespace unity
+
+universe variable u
+
+class has_safety (α : Type u) : Type (u+1) :=
+  (σ : Type)
+  (step : α → σ → σ → Prop)
+
+def state := has_safety.σ
+
+def pred α [has_safety α] := state α → Prop
+
+def unless {α} [has_safety α] (s : α) (p q : pred α) : Prop
+:= ∀ σ σ', has_safety.step s σ σ' → p σ ∧ ¬ q σ → p σ' ∨ q σ'
+
+section properties
+
+open predicate
+
+parameter {α : Type u}
+variable [has_safety α]
+variable s : α
+def σ := state α
+
+lemma impl_unless {p q : pred' σ} (h : ∀ i, p i → q i) : unless s p q :=
+begin
+  intros σ σ' h₀ h₁,
+  cases h₁ with h₁ h₂,
+  cases h₂ (h _ h₁)
+end
+
+lemma unless_weak_rhs {p q r : pred' σ}
+         (h : ∀ i, q i → r i)
+         (P₀ : unless s p q)
+         : unless s p r :=
+begin
+  apply forall_imp_forall _ P₀,
+  intro s,
+  apply forall_imp_forall _,
+  intro s',
+  apply imp_imp_imp_right' _,
+  intro step,
+  apply imp_mono,
+  { apply and.imp id,
+    apply imp_imp_imp_left,
+    apply h },
+  { apply or.imp_right,
+    apply h }
+end
+
+lemma unless_conj_gen {p₀ q₀ p₁ q₁ : pred' σ}
+         (P₀ : unless s p₀ q₀)
+         (P₁ : unless s p₁ q₁)
+         : unless s (p₀ && p₁) ((q₀ && p₁) || (p₀ && q₁) || (q₀ && q₁)) :=
+begin
+  intros s s' step H,
+  note P₀ := P₀ s s' step,
+  note P₁ := P₁ s s' step,
+  cases H with H₀ H₂,
+  cases H₀ with Hp₀ Hp₁,
+  simp [not_or_iff_not_and_not,not_and_iff_not_or_not] at H₂,
+  cases H₂ with Hnpnq H₂, cases H₂ with Hnqnp Hnqnq,
+  assert Hnq₀ : ¬ q₀ s,
+  { cases Hnqnp with h h, assumption,
+    cases h Hp₁ },
+  assert Hnq₁ : ¬ q₁ s,
+  { cases Hnpnq with h h,
+    cases h Hp₀,
+    apply h },
+  note P₀ := P₀ ⟨Hp₀,Hnq₀⟩,
+  note P₁ := P₁ ⟨Hp₁,Hnq₁⟩,
+  cases P₀ with P₀ P₀
+  ; cases P₁ with P₁ P₁,
+  { left, exact ⟨P₀,P₁⟩ },
+  { apply or.inr (or.inl $ or.inr _),
+    exact ⟨P₀,P₁⟩ },
+  { apply or.inr (or.inl $ or.inl _),
+    exact ⟨P₀,P₁⟩ },
+  { apply or.inr (or.inr _),
+    exact ⟨P₀,P₁⟩ },
+end
+
+end properties
+
+end unity
